theories/iris/language/lwp_resources.v
@@ -10,10 +10,6 @@ Section lwp_resources.
   Context `{!wasmG Σ}.
   Open Scope bi_scope.
 
-Locate Wasm.iris.language.iris.iris.val.
-Locate iris.val.
-Locate Wasm.iris.language.iris.iris.val.
-
   Lemma lenient_wp_get_local s E (v: value) i Φ f :
     (f_locs f) !! i = Some v ->
     ▷Φ.(lp_val) [v] ∗
@@ -34,36 +30,6 @@ Locate Wasm.iris.language.iris.iris.val.
       iFrame.
   Qed.
 
-  Check wp_set_local.
-
-  Definition lp_fr_set f i v (Φ : @logpred Σ) : logpred :=
-    {|
-      lp_fr := λ f', ⌜f' = {| f_locs := seq.set_nth v (f_locs f) i v; f_inst := f_inst f |}⌝;
-      lp_val := lp_val Φ;
-      lp_trap := lp_trap Φ;
-      lp_br := lp_br Φ;
-      lp_ret := lp_ret Φ;
-      lp_host := lp_host Φ;
-    |}.
-
-  Definition lp_run Φ :=
-    {|
-      lp_fr := lp_fr Φ;
-      lp_val := λ vs, lp_val Φ vs ∗ ↪[RUN];
-      lp_trap := lp_trap Φ;
-      lp_br := λ x, lp_br Φ x ∗ ↪[RUN];
-      lp_ret := λ x, lp_ret Φ x ∗ ↪[RUN];
-      lp_host := λ ft hf vs lh, lp_host Φ ft hf vs lh ∗ ↪[RUN];
-    |}.
-
-  Lemma lp_run_sep Φ w :
-    denote_logpred Φ w ∗ ↪[RUN] ⊢ denote_logpred (lp_run Φ) w.
-  Proof.
-    unfold lp_run, denote_logpred.
-    cbn.
-    destruct w; cbn; iIntros "[HΦ Hrun]"; iFrame.
-  Qed.
-
   Lemma lenient_wp_set_local s E i Φ v (f: datatypes.frame) :
     i < length f.(f_locs) ->
     ▷ Φ.(lp_val) [] ∗
@@ -78,8 +44,67 @@ Locate Wasm.iris.language.iris.iris.val.
     - instantiate (1:= lp_noframe (lp_fr_set f i v Φ)).
       by cbn.
     - iIntros (w) "((Hpred & Hrun) & Hf)".
-      iApply lp_run_sep.
+      iApply lp_with_sep.
       by iFrame.
+  Qed.
+
+  Theorem lenient_wp_tee_local s E i Φ v (f: datatypes.frame) :
+    i < length f.(f_locs) ->
+    ↪[frame] f ∗
+    ↪[RUN] ∗
+    ▷ (↪[frame] f -∗
+        ↪[RUN] -∗
+        lenient_wp s E [AI_basic (BI_const v); AI_basic (BI_const v); AI_basic (BI_set_local i)] Φ)
+    ⊢ lenient_wp s E [AI_basic (BI_const v); AI_basic (BI_tee_local i)] Φ.
+  Proof.
+    iIntros (Hlocs) "(Hf & Hr & Hwp)".
+    iApply (wp_tee_local with "[$] [$] [$]").
+  Qed.
+
+  Theorem lenient_wp_load Φ s E t v off a k n f i : 
+    let R := N.of_nat n ↦[wms][Wasm_int.N_of_uint i32m k + off] bits v in
+    is_true (types_agree t v) ->
+    inst_memory (f_inst f) !! i = Some n ->
+    R ∗
+    ↪[RUN] ∗
+    ▷ Φ.(lp_val) [v] ∗
+    Φ.(lp_fr) f ∗
+    ↪[frame] f
+    ⊢ lenient_wp s E [AI_basic (BI_const (VAL_int32 k)); AI_basic (BI_load i t None a off)]
+                     (lp_with (R ∗ ↪[RUN]) Φ).
+  Proof.
+    iIntros (R Hag Hmem) "(Hwp & Hrun & Hval & Hfr & Hf)".
+    iApply (wp_wand with "[Hwp Hrun Hval Hfr Hf]").
+    iApply wp_load; eauto.
+    - iFrame.
+      instantiate (1:=(fun v: iris.val => (lp_noframe Φ v ∗ lp_fr Φ f)%I)).
+      iFrame.
+    - iIntros (v0) "[[[Hnoframe Hfr] [HR Hrun]] Hf]".
+      rewrite -lp_with_sep.
+      iFrame.
+  Qed.
+
+  Theorem lenient_wp_store Φ s E t bs v off a k n f i :
+    is_true (types_agree t v) ->
+    length bs = length_t t ->
+    inst_memory (f_inst f) !! i = Some n ->
+    N.of_nat n↦[wms][Wasm_int.N_of_uint i32m k + off] bs ∗
+    ↪[RUN] ∗
+    ▷ Φ.(lp_val) [] ∗
+    Φ.(lp_fr) f ∗
+    ↪[frame] f
+    ⊢ lenient_wp s E [AI_basic (BI_const (VAL_int32 k)); AI_basic (BI_const v); AI_basic (BI_store i t None a off)]
+                     (lp_with (N.of_nat n↦[wms][Wasm_int.N_of_uint i32m k + off]bits v ∗ ↪[RUN]) Φ).
+  Proof.
+    iIntros (Hag Hlen Hmem) "(Hptr & Hrun & Hval & Hfr & Hf)".
+    iApply (wp_wand with "[Hptr Hrun Hval Hf]").
+    - iFrame.
+      iApply wp_store; eauto.
+      instantiate (1:=(fun v: iris.val => lp_noframe Φ v)).
+      iFrame.
+    - iIntros (v0) "[[Hnofram [Hptr Hrun]] Hf]".
+      rewrite -lp_with_sep.
+      iFrame.
   Qed.
 
 End lwp_resources.
